Utlc/LemmasEvaluation.v
@@ -29,11 +29,10 @@ Section SubstEval.
   Proof. induction C; crushUtlc. Qed.
   Hint Resolve ectx_sub.
 
-  Lemma eval_closed_under_substitution {t1 t2} (r: t1 --> t2) :
-    ∀ (ζ: Sub UTm), t1[ζ] --> t2[ζ].
+  Lemma eval₀_closed_under_substitution {t1 t2} (r: t1 -->₀ t2) :
+    ∀ (ζ: Sub UTm), t1[ζ] -->₀ t2[ζ].
   Proof.
-    induction r; crushUtlc; eauto with eval; unfold not in *.
-    - constructor; destruct C; crushUtlc.
+    induction r; crushUtlc; eauto with eval; unfold not in *. 
     - constructor; destruct t₁; crushUtlc.
     - constructor; destruct t₁; crushUtlc.
     - constructor; destruct t; crushUtlc.
@@ -41,4 +40,79 @@ Section SubstEval.
     - constructor; destruct t; crushUtlc.
   Qed.
 
+  Lemma eval_closed_under_substitution {t1 t2} (r: t1 --> t2) (ζ: Sub UTm) :
+    t1[ζ] --> t2[ζ].
+  Proof.
+    induction r as [C t₁' t₂' e₀|C]; rewrite -> ?pctx_app_sub.
+    - assert (t₁'[ζ ↑⋆ depthPCtx C] -->₀ t₂'[ζ ↑⋆ depthPCtx C]); eauto using eval₀_closed_under_substitution with eval. 
+    - constructor; induction C; crushUtlc.  
+  Qed.
+
 End SubstEval.
+
+Lemma ectx_cat (C₁ C₂: PCtx) :
+  ECtx C₁ → ECtx C₂ → ECtx (pctx_cat C₁ C₂).
+Proof.
+  induction C₂; simpl; intros; destruct_conjs; auto.
+Qed.
+
+Lemma pctx_cat_app (t : UTm) (C₁ C₂ : PCtx) :
+  pctx_app t (pctx_cat C₁ C₂) = pctx_app (pctx_app t C₁) C₂.
+Proof.
+  induction C₂; crushUtlc.
+Qed.
+
+(* The following doesn't hold here: C[wrong] evaluates to wrong in single step *)
+(* Lemma eval_ctx {C t t'}  : t --> t' -> ECtx C -> pctx_app t C --> pctx_app t' C. *)
+(* Proof. *)
+(*   induction 1. *)
+(*   rewrite <- ?pctx_cat_app in *. *)
+(*   eauto using ectx_cat with eval. *)
+(* Qed. *)
+  
+Lemma ectx_wrong_not_value {C} : ECtx C -> not (Value (pctx_app wrong C)).
+Proof.
+  intros ec val.
+  induction C; crushUtlc.
+Qed.
+
+Lemma values_are_normal {t : UTm} : Value t -> normal t.
+Proof.
+  intros  vt.
+  induction t; simpl in vt; try match goal with [ H : False |- _ ] => destruct H end; try eauto; intro et'; destruct et' as [t' et'];
+  depind et'; induction C; crushUtlc;
+  repeat try match goal with 
+      | [ H : abs _ -->₀ _ |- _] => depind H
+      | [ H : unit -->₀ _ |- _] => depind H
+      | [ H : true -->₀ _ |- _] => depind H
+      | [ H : false -->₀ _ |- _] => depind H
+      | [ H : pair _ _ -->₀ _ |- _] => depind H
+      | [ H : inl _ -->₀ _ |- _] => depind H
+      | [ H : inr _ -->₀ _ |- _] => depind H
+      | [ H : pair _ _ = pair _ _ |- _] => inversion H; clear H; subst
+      | [ H : inl _ = inl _ |- _] => inversion H; clear H; subst
+      | [ H : inr _ = inr _ |- _] => inversion H; clear H; subst
+      | [ H : _ ∧ _ |- _] => destruct_conjs
+      | [ H : Value (pctx_app wrong _) |- _] => exfalso; refine (ectx_wrong_not_value _ H); auto
+  end.
+  - apply IHt1; [assumption| exists (pctx_app t' C); eauto with eval].
+  - apply IHt2; [assumption| exists (pctx_app t' C); eauto with eval].
+  - apply IHt; [assumption| exists (pctx_app t' C); eauto with eval].
+  - apply IHt; [assumption| exists (pctx_app t' C); eauto with eval].
+Qed.
+
+Lemma TerminatingDN (t: UTm) n (m: t ⇓_ (S n)) :
+  ∀ t', t --> t' → TerminatingN t' n.
+Proof. 
+  depind m; intros t' e'; eauto using values_are_normal.
+  exfalso.
+  refine (values_are_normal H _); exists t'; auto.
+Qed.
+
+
+Lemma TerminatingN_Terminating {t : UTm} {n} : t ⇓_ n -> t ⇓.
+Proof.
+  induction 1; constructor; try assumption.
+  intros t' e'. exfalso. refine (values_are_normal H _).
+  exists t'. auto.
+Qed.
